src/Regions.v
@@ -4,7 +4,8 @@ Require Import Coq.FSets.FMapInterface.
 
 Module Regions (Map : WSfun).
 
-Include Heap Map.
+Module Heap := Heap Map.
+Export Heap.
 
 Module SomeAddrMap := Map DecidableSomeAddr.
 Definition someAddrMap := SomeAddrMap.t.
@@ -84,11 +85,12 @@ End Regions.
 
 Module WellFormedHeaps (Map : WSfun).
 
-Include Regions Map.
-
-Module Program := Program Map.
+Module Regions := Regions Map.
+Export Regions.
 
 Module Typing := Typing Map.
+Import Typing. 
+Import Typing.Context.
 
 Inductive values_typed (chi : heap) (r : regPart chi) (iota : someAddr) : list value -> list accessor -> list Syntax.aliasedType -> Prop :=
   | values_typed_nil
@@ -100,16 +102,16 @@ Inductive values_typed (chi : heap) (r : regPart chi) (iota : someAddr) : list v
     -> values_typed chi r iota lv la lt 
     -> values_typed chi r iota (v :: lv) (a :: la) ((Syntax.aType s b) :: lt).
 
-Inductive well_formed_message { p : Program.program } (chi : heap) (r : regPart chi) : option messageAddr -> Syntax.actorId -> Prop :=
+Inductive well_formed_message { p : program } (chi : heap) (r : regPart chi) : option messageAddr -> Syntax.actorId -> Prop :=
   | wf_message (iota : messageAddr) (rcvrId : Syntax.actorId) (bId : Syntax.behaviourId) (mArgs : list value) (mNext : option messageAddr)
-      (bArgs : Program.arrayVarMap Syntax.aliasedType) (bBody : Syntax.expressionSeq)
+      (bArgs : arrayVarMap Syntax.aliasedType) (bBody : Syntax.expressionSeq)
   : HeapMapsTo message (someMessageAddr iota) (messageAlloc bId mArgs mNext) chi
-    -> @Program.behaviourLookup p (inr rcvrId)  bId (Program.bDef bArgs bBody) 
+    -> @behaviourLookup p (inr rcvrId)  bId (bDef bArgs bBody) 
     -> perspJudgement chi r (someMessageAddr iota) next (option_map someMessageAddr mNext) Syntax.iso
     -> values_typed chi r (someMessageAddr iota)
           mArgs
-          (map varAcc (map fst (Program.ArrayVarMap.elements bArgs)))
-          (map snd (Program.ArrayVarMap.elements bArgs))
+          (map varAcc (map fst (ArrayVarMap.elements bArgs)))
+          (map snd (ArrayVarMap.elements bArgs))
     -> well_formed_message chi r mNext rcvrId
     -> well_formed_message chi r (Some iota) rcvrId
   | wf_message_nul (a : Syntax.actorId)
@@ -117,7 +119,7 @@ Inductive well_formed_message { p : Program.program } (chi : heap) (r : regPart 
 
 Inductive well_formed_frame (chi : heap) (r : regPart chi) : option frameAddr -> Prop :=
   (* TODO: This is not complete *)
-  | wf_frame_top (iota : frameAddr) (gamma : Typing.context) (L : localVars) (E : Syntax.expressionSeq) (v_super : frameAddr?)
+  | wf_frame_top (iota : frameAddr) (gamma : context) (L : localVars) (E : Syntax.expressionSeq) (v_super : frameAddr?)
   : HeapMapsTo frame (someFrameAddr iota) (frameAlloc L E None v_super) chi
     -> False (* TODO: check local variables are well-typed w.r.t. something *)
     -> False (* TODO: check the return type is good for the superframe *)
@@ -127,7 +129,7 @@ Inductive well_formed_frame (chi : heap) (r : regPart chi) : option frameAddr ->
   : well_formed_frame chi r None
 with
 well_formed_frame_if_returned (chi : heap) (r : regPart chi) : option frameAddr -> Syntax.ponyType -> Prop :=
-  | wf_frame_ir (iota : frameAddr) (gamma : Typing.context) (L : localVars) (E : Syntax.expressionSeq) (v_super : frameAddr?)
+  | wf_frame_ir (iota : frameAddr) (gamma : context) (L : localVars) (E : Syntax.expressionSeq) (v_super : frameAddr?)
       (t : Syntax.ponyType)
   : HeapMapsTo frame (someFrameAddr iota) (frameAlloc L E None v_super) chi
     -> False (* TODO: check local variables are well-typed w.r.t. something *)
